theories/program_logic/lifting.v
@@ -3,8 +3,8 @@ From diris.program_logic Require Export weakestpre.
 Set Default Proof Using "Type".
 
 Section lifting.
-Context `{!irisG Λ Σ}.
-Implicit Types s : stuckness.
+Context `{!irisG Λ Σ ξ}.
+Implicit Types s : ξ.
 Implicit Types v : val Λ.
 Implicit Types e : expr Λ.
 Implicit Types σ : state Λ.
@@ -13,22 +13,24 @@ Implicit Types Φ : val Λ → iProp Σ.
 
 Hint Resolve reducible_no_obs_reducible : core.
 
-Lemma wp_lift_step_fupd s i E Φ e1 :
+Lemma wp_lift_step_fupd s E Φ e1 :
   to_val e1 = None →
-  (∀ σ1 κ κs es, state_interp σ1 (κ ++ κs) es ={E,∅}=∗
-    ⌜if s is NotStuck then reducible e1 σ1 ∨ waiting e1 σ1 else True⌝ ∗
-    ∀ e2 σ2 efs, ⌜prim_step e1 σ1 κ e2 σ2 efs⌝ ={∅,∅,E}▷=∗
-      state_interp σ2 κs ((<[i := e2]> es) ++ efs) ∗
-      WP e2 @ (s,i); E {{ Φ }} ∗
-      [∗ list] i ↦ ef ∈ efs, WP ef @ (s,length es + i); ⊤ {{ fork_post (length es + i) }})
-  ⊢ WP e1 @ (s,i); E {{ Φ }}.
+  (∀ ζ σ1 κ κs es tid,
+     ⌜ tid_get s tid ∧ es !! tid = Some e1 ⌝ -∗
+     state_interp ζ σ1 (κ ++ κs) es ={E,∅}=∗
+       ⌜ state_valid ζ σ1 s e1 ⌝ ∧
+       ∀ e2 σ2 efs,
+         ⌜ prim_step e1 σ1 κ e2 σ2 efs ⌝ ={∅,∅,E}▷=∗
+         ∃ ζ', state_interp ζ' σ2 κs (<[tid:=e2]> es ++ efs) ∗
+          WP e2 @ s ; E {{ Φ }} ∗
+          [∗ list] i ↦ ef ∈ efs,
+            WP ef @ (tid_set (i + length es) s) ; ⊤ {{ fork_post (i + length es) }})
+  ⊢ WP e1 @ s; E {{ Φ }}.
 Proof.
-  rewrite wp_unfold /wp_pre=>->. iIntros "H" (σ1 κ κs es) "Hf Hσ".
-  iMod ("H" with "Hσ") as "(%&H)". iModIntro. iSplit. by destruct s.
-  iIntros (????). iApply "H". eauto.
+  by rewrite wp_unfold /wp_pre=>->.
 Qed.
 
-Lemma wp_lift_stuck E Φ e i :
+(* Lemma wp_lift_stuck E Φ e i :
   to_val e = None →
   (∀ σ κs es, state_interp σ κs es ={E,∅}=∗ ⌜stuck e σ⌝)
   ⊢ WP e @ (MaybeStuck,i); E {{ Φ }}.
@@ -38,10 +40,10 @@ Proof.
   iIntros (e2 σ2 efs ?).
   destruct Hirr as [Hirr H1].
   by case: (Hirr κ e2 σ2 efs).
-Qed.
+Qed. *)
 
 (** Derived lifting lemmas. *)
-Lemma wp_lift_step s i E Φ e1 :
+(* Lemma wp_lift_step s E Φ e1 :
   to_val e1 = None →
   (∀ σ1 κ κs es, state_interp σ1 (κ ++ κs) es ={E,∅}=∗
     ⌜if s is NotStuck then reducible e1 σ1 ∨ waiting e1 σ1 else True⌝ ∗
@@ -53,15 +55,44 @@ Lemma wp_lift_step s i E Φ e1 :
 Proof.
   iIntros (?) "H". iApply wp_lift_step_fupd; [done|]. iIntros (????) "Hσ".
   iMod ("H" with "Hσ") as "[$ H]". iIntros "!> * % !> !>". by iApply "H".
+Qed. *)
+
+
+(* state_valid : abstract_state → state Λ → A → expr Λ → Prop; *)
+Lemma wp_lift_pure_step_no_fork `{!Inhabited (state Λ)} s E E' Φ e1 :
+  to_val e1 = None →
+  (∀ ζ σ1, state_valid ζ σ1 s e1) →
+  (∀ κ κs σ1 e2 σ2 efs es i  ζ, tid_get s i → prim_step e1 σ1 κ e2 σ2 efs → κ = [] ∧ σ2 = σ1 ∧ efs = [] ∧
+    (state_interp ζ σ1 κs (<[i:=e1]> es) ⊢ state_interp ζ σ2 κs (<[i:=e2]> es))) →
+  (|={E,E'}▷=> ∀ κ e2 efs σ, ⌜prim_step e1 σ κ e2 σ efs⌝ → WP e2 @ s; E {{ Φ }})
+  ⊢ WP e1 @ s; E {{ Φ }}.
+Proof.
+  iIntros (Hnoval Hvalid Hstep) "H".
+  iApply wp_lift_step_fupd; first done.
+  iIntros (ζ σ1 κ κs es tid [tidg tidh]) "Hsi".
+  iMod "H".
+  iMod (fupd_intro_mask' E' ∅) as "Hclose"; first by apply empty_subseteq.
+  iModIntro.
+  iSplit; first done.
+  iIntros (e2 σ2 efs primst).
+  destruct (Hstep κ κs σ1 e2 σ2 efs es tid ζ) as (-> & <- & -> & Hsi);[done..|].
+  iMod "Hclose" as "_".
+  iExists ζ. simpl.
+  replace (state_interp ζ σ2 κs es) with (state_interp ζ σ2 κs (<[tid:=e1]> es)) by
+    (rewrite list_insert_id; auto).
+  rewrite app_nil_r.
+  iMod (fupd_intro_mask' _ ∅) as "Hclose"; first by apply empty_subseteq.
+  iModIntro. iNext.
+  iMod "Hclose" as "_".
+  iMod "H".
+  iModIntro.
+  iSplitL "Hsi"; first by iApply Hsi.
+  iSplitL; last done.
+  by iApply "H".
 Qed.
 
-Lemma wp_lift_pure_step_no_fork `{!Inhabited (state Λ)} s i E E' Φ e1 :
-  (∀ σ1, if s is NotStuck then reducible e1 σ1 ∨ waiting e1 σ1 else to_val e1 = None) →
-  (∀ κ σ1 e2 σ2 efs, prim_step e1 σ1 κ e2 σ2 efs → κ = [] ∧ σ2 = σ1 ∧ efs = []) →
-  (|={E,E'}▷=> ∀ κ e2 efs σ, ⌜prim_step e1 σ κ e2 σ efs⌝ → WP e2 @ (s,i); E {{ Φ }})
-  ⊢ WP e1 @ (s,i); E {{ Φ }}.
-Proof.
-  iIntros (Hsafe Hstep) "H". iApply wp_lift_step.
+
+(* iIntros (Hsafe Hstep) "H". iApply wp_lift_step.
   { specialize (Hsafe inhabitant).
     destruct s; naive_solver eauto using reducible_not_val, waiting_not_val. }
   iIntros (σ1 κ κs es) "Hσ". iMod "H".
@@ -71,8 +102,9 @@ Proof.
   destruct (Hstep κ σ1 e2 σ2 efs) as (-> & <- & ->); auto.
   iMod "Hclose" as "_". iMod "H". iModIntro.
   iDestruct ("H" with "[//]") as "H". simpl. rewrite app_nil_r. iFrame.
-Admitted.
+Admitted. *)
 
+(*
 Lemma wp_lift_pure_stuck `{!Inhabited (state Λ)} E Φ e i :
   (∀ σ, stuck e σ) →
   True ⊢ WP e @ (MaybeStuck,i); E {{ Φ }}.
@@ -81,32 +113,38 @@ Proof.
   - destruct(to_val e) as [v|] eqn:He; last done.
     rewrite -He. by case: (Hstuck inhabitant).
   - iIntros (σ κs n) "_". by iMod (fupd_intro_mask' E ∅) as "_"; first set_solver.
-Qed.
+Qed. *)
 
 (* Atomic steps don't need any mask-changing business here, one can
    use the generic lemmas here. *)
 Lemma wp_lift_atomic_step_fupd {s i E1 E2 Φ} e1 :
+  tid_get s i →
   to_val e1 = None →
-  (∀ σ1 κ κs es, state_interp σ1 (κ ++ κs) es ={E1}=∗
-    ⌜if s is NotStuck then reducible e1 σ1 ∨ waiting e1 σ1 else True⌝ ∗
+  (∀ ζ σ1 κ κs es, state_interp ζ σ1 (κ ++ κs) es ={E1}=∗
+    ⌜state_valid ζ σ1 s e1⌝ ∗
     ∀ e2 σ2 efs, ⌜prim_step e1 σ1 κ e2 σ2 efs⌝ ={E1,E2}▷=∗
-      state_interp σ2 κs ((<[i := e2]> es) ++ efs) ∗
+      ∃ ζ', state_interp ζ' σ2 κs ((<[i := e2]> es) ++ efs) ∗
       from_option Φ False (to_val e2) ∗
-      [∗ list] i ↦ ef ∈ efs, WP ef @ (s,length es + i); ⊤ {{ fork_post (length es + i) }})
-  ⊢ WP e1 @ (s,i); E1 {{ Φ }}.
+      [∗ list] i ↦ ef ∈ efs, WP ef @ (tid_set (i + length es) s); ⊤ {{ fork_post (i + length es) }})
+  ⊢ WP e1 @ s; E1 {{ Φ }}.
 Proof.
-  iIntros (?) "H".
-  iApply (wp_lift_step_fupd s i E1 _ e1) =>//; iIntros (σ1 κ κs es) "Hσ1".
-  iMod ("H" $! σ1 with "Hσ1") as "[$ H]".
-  iMod (fupd_intro_mask' E1 ∅) as "Hclose"; first set_solver.
-  iIntros "!>" (e2 σ2 efs ?). iMod "Hclose" as "_".
-  iMod ("H" $! e2 σ2 efs with "[#]") as "H"; [done|].
+  iIntros (tidg1 ?) "H".
+  iApply wp_lift_step_fupd; first done.
+  iIntros (ζ σ1 κ κs es tid [tidg2 tidh]) "Hsi".
+  pose proof (tid_func _ _ _ tidg1 tidg2). subst.
+  iMod ("H" with "Hsi") as "[$ H]".
+  iMod (fupd_intro_mask' E1 ∅) as "Hclose"; first by apply empty_subseteq.
+  iModIntro. iIntros (e2 σ2 efs Hps).
+  iMod "Hclose" as "_".
+  iMod ("H" with "[//]") as "H".
   iMod (fupd_intro_mask' E2 ∅) as "Hclose"; [set_solver|]. iIntros "!> !>".
-  iMod "Hclose" as "_". iMod "H" as "($ & HQ & $)".
-  destruct (to_val e2) eqn:?; last by iExFalso.
+  iMod "Hclose" as "_". iMod "H" as (ζ') "(Hsi & Hfo & Hr)".
+  destruct (to_val e2) eqn:?; last by iExFalso. simpl.
+  iExists ζ'. iFrame.
   iApply wp_value; last done. by apply of_to_val.
 Qed.
 
+(*
 Lemma wp_lift_atomic_step {s i E Φ} e1 :
   to_val e1 = None →
   (∀ σ1 κ κs es, state_interp σ1 (κ ++ κs) es ={E}=∗
@@ -121,7 +159,7 @@ Proof.
   iIntros (????) "?". iMod ("H" with "[$]") as "[$ H]".
   iIntros "!> *". iIntros (Hstep) "!> !>".
   by iApply "H".
-Qed.
+Qed. *)
 
 Lemma wp_lift_pure_det_step_no_fork `{!Inhabited (state Λ)} {s i E E' Φ} e1 e2 :
   (∀ σ1, if s is NotStuck then reducible e1 σ1 ∨ waiting e1 σ1 else to_val e1 = None) →
